wip

chacha20-rust/src/bounded_index.rs
@@ -1,0 +1,17 @@
+// #[derive(Copy, Clone)]
+// pub struct BoundedIndex<const MAX: usize>(pub usize);
+
+// use std::ops::{Index, IndexMut};
+
+// impl<const MAX: usize, T> Index<BoundedIndex<MAX>> for [T; MAX] {
+//     type Output = T;
+//     fn index(&self, BoundedIndex(i): BoundedIndex<MAX>) -> &T {
+//         self.index(i)
+//     }
+// }
+
+// impl<const MAX: usize, T> IndexMut<BoundedIndex<MAX>> for [T; MAX] {
+//     fn index_mut(&mut self, BoundedIndex(i): BoundedIndex<MAX>) -> &mut T {
+//         self.index_mut(i)
+//     }
+// }
