chacha20-rust/out/Core.Iter.Traits.Collect.IntoIterator.fst
@@ -1,1 +1,3 @@
 module Core.Iter.Traits.Collect.IntoIterator
+
+let into_iter = id
