chacha20-rust/out/Chacha20.Bounded_index.fst
@@ -1,0 +1,5 @@
+module Chacha20.Bounded_index
+#set-options "--fuel 0 --ifuel 1 --z3rlimit 15"
+open Core
+
+type t_BoundedIndex = | BoundedIndex : usize -> t_BoundedIndex
