chacha20-rust/out/Core.Iter.Traits.Iterator.Iterator.fst
@@ -1,11 +1,3 @@
 module Core.Iter.Traits.Iterator.Iterator
 
-open Core.Types
-
-class tc self = {
-  item: Type;
-  next: self -> self * option item;
-  size_hint: self -> option usize;
-  fold: b:Type -> self -> b -> (b -> item -> b) -> b
-}
-
+include Core.Iter
