chacha20/out/Hacspec_chacha20.To_be_bytes.fst
@@ -1,0 +1,15 @@
+module Hacspec_chacha20.To_be_bytes
+#set-options "--fuel 0 --ifuel 1 --z3rlimit 15"
+open FStar.Mul
+open Hacspec.Lib
+open Hacspec_lib_tc
+
+let fACTOR: uint_size = Core.Mem.size_of
+
+let fACTOR: uint_size = Core.Mem.size_of
+
+let fACTOR: uint_size = Core.Mem.size_of
+
+let fACTOR: uint_size = Core.Mem.size_of
+
+let fACTOR: uint_size = Core.Mem.size_of
