sha256-rust/out/Chacha20.Hacspec_helper.fst
@@ -1,0 +1,137 @@
+module Chacha20.Hacspec_helper
+#set-options "--fuel 0 --ifuel 1 --z3rlimit 15"
+open Core
+
+let to_le_u32s_3_ (bytes: slice u8) : array u32 3sz =
+  let _:never =
+    match 3sz, Core.Slice.len_under_impl bytes /. 4sz with
+    | left_val, right_val ->
+      if ~.(left_val =. right_val)
+      then
+        let kind:Core.Panicking.t_AssertKind = Core.Panicking.AssertKind_Eq in
+        Core.Panicking.assert_failed kind left_val right_val Core.Option.Option_None
+  in
+  let out:array u32 3sz = Hax.Array.repeat 0ul 3sz in
+  let out:array u32 3sz =
+    Core.Iter.Traits.Iterator.Iterator.fold (Core.Iter.Traits.Collect.IntoIterator.into_iter ({
+              Core.Ops.Range.Range.f_start = 0sz;
+              Core.Ops.Range.Range.f_end = 3sz
+            }))
+      out
+      (fun out i ->
+          out.[ i ] <-
+            Core.Num.from_le_bytes_under_impl_8 (Core.Result.unwrap_under_impl (Core.Convert.TryInto.try_into
+                      bytes.[ {
+                          Core.Ops.Range.Range.f_start = 4sz *. i;
+                          Core.Ops.Range.Range.f_end = 4sz *. i +. 4sz
+                        } ])))
+  in
+  out
+
+let to_le_u32s_8_ (bytes: slice u8) : array u32 8sz =
+  let _:never =
+    match 8sz, Core.Slice.len_under_impl bytes /. 4sz with
+    | left_val, right_val ->
+      if ~.(left_val =. right_val)
+      then
+        let kind:Core.Panicking.t_AssertKind = Core.Panicking.AssertKind_Eq in
+        Core.Panicking.assert_failed kind left_val right_val Core.Option.Option_None
+  in
+  let out:array u32 8sz = Hax.Array.repeat 0ul 8sz in
+  let out:array u32 8sz =
+    Core.Iter.Traits.Iterator.Iterator.fold (Core.Iter.Traits.Collect.IntoIterator.into_iter ({
+              Core.Ops.Range.Range.f_start = 0sz;
+              Core.Ops.Range.Range.f_end = 8sz
+            }))
+      out
+      (fun out i ->
+          out.[ i ] <-
+            Core.Num.from_le_bytes_under_impl_8 (Core.Result.unwrap_under_impl (Core.Convert.TryInto.try_into
+                      bytes.[ {
+                          Core.Ops.Range.Range.f_start = 4sz *. i;
+                          Core.Ops.Range.Range.f_end = 4sz *. i +. 4sz
+                        } ])))
+  in
+  out
+
+let to_le_u32s_16_ (bytes: slice u8) : array u32 16sz =
+  let _:never =
+    match 16sz, Core.Slice.len_under_impl bytes /. 4sz with
+    | left_val, right_val ->
+      if ~.(left_val =. right_val)
+      then
+        let kind:Core.Panicking.t_AssertKind = Core.Panicking.AssertKind_Eq in
+        Core.Panicking.assert_failed kind left_val right_val Core.Option.Option_None
+  in
+  let out:array u32 16sz = Hax.Array.repeat 0ul 16sz in
+  let out:array u32 16sz =
+    Core.Iter.Traits.Iterator.Iterator.fold (Core.Iter.Traits.Collect.IntoIterator.into_iter ({
+              Core.Ops.Range.Range.f_start = 0sz;
+              Core.Ops.Range.Range.f_end = 16sz
+            }))
+      out
+      (fun out i ->
+          out.[ i ] <-
+            Core.Num.from_le_bytes_under_impl_8 (Core.Result.unwrap_under_impl (Core.Convert.TryInto.try_into
+                      bytes.[ {
+                          Core.Ops.Range.Range.f_start = 4sz *. i;
+                          Core.Ops.Range.Range.f_end = 4sz *. i +. 4sz
+                        } ])))
+  in
+  out
+
+let u32s_to_le_bytes (state: array u32 16sz) : array u8 64sz =
+  let out:array u8 64sz = Hax.Array.repeat 0uy 64sz in
+  let out:array u8 64sz =
+    Core.Iter.Traits.Iterator.Iterator.fold (Core.Iter.Traits.Collect.IntoIterator.into_iter ({
+              Core.Ops.Range.Range.f_start = 0sz;
+              Core.Ops.Range.Range.f_end = Core.Slice.len_under_impl (Hax.CoerceUnsize.unsize state)
+            }))
+      out
+      (fun out i ->
+          let tmp:array u8 4sz = Core.Num.to_le_bytes_under_impl_8 state.[ i ] in
+          Core.Iter.Traits.Iterator.Iterator.fold (Core.Iter.Traits.Collect.IntoIterator.into_iter ({
+                    Core.Ops.Range.Range.f_start = 0sz;
+                    Core.Ops.Range.Range.f_end = 4sz
+                  }))
+            out
+            (fun out j -> out.[ i *. 4sz +. j ] <- tmp.[ j ]))
+  in
+  out
+
+let xor_state (state other: array u32 16sz) : array u32 16sz =
+  let state:array u32 16sz =
+    Core.Iter.Traits.Iterator.Iterator.fold (Core.Iter.Traits.Collect.IntoIterator.into_iter ({
+              Core.Ops.Range.Range.f_start = 0sz;
+              Core.Ops.Range.Range.f_end = 16sz
+            }))
+      state
+      (fun state i -> state.[ i ] <- state.[ i ] ^. other.[ i ])
+  in
+  state
+
+let add_state (state other: array u32 16sz) : array u32 16sz =
+  let state:array u32 16sz =
+    Core.Iter.Traits.Iterator.Iterator.fold (Core.Iter.Traits.Collect.IntoIterator.into_iter ({
+              Core.Ops.Range.Range.f_start = 0sz;
+              Core.Ops.Range.Range.f_end = 16sz
+            }))
+      state
+      (fun state i -> state.[ i ] <- Core.Num.wrapping_add_under_impl_8 state.[ i ] other.[ i ])
+  in
+  state
+
+let update_array (array: array u8 64sz) (val: slice u8) : array u8 64sz =
+  let _:never =
+    if ~.(64sz >=. Core.Slice.len_under_impl val)
+    then Core.Panicking.panic "assertion failed: 64 >= val.len()"
+  in
+  let array:array u8 64sz =
+    Core.Iter.Traits.Iterator.Iterator.fold (Core.Iter.Traits.Collect.IntoIterator.into_iter ({
+              Core.Ops.Range.Range.f_start = 0sz;
+              Core.Ops.Range.Range.f_end = Core.Slice.len_under_impl val
+            }))
+      array
+      (fun array i -> array.[ i ] <- val.[ i ])
+  in
+  array
