sha256-rust/out/Chacha20.fst
@@ -1,0 +1,194 @@
+module Chacha20
+#set-options "--fuel 0 --ifuel 1 --z3rlimit 15"
+open Core
+
+let t_State = array u32 16sz
+
+let t_Block = array u8 64sz
+
+let t_ChaChaIV = array u8 12sz
+
+let t_ChaChaKey = array u8 32sz
+
+let t_StateIdx = usize
+
+let v_BoundedIndex (x: usize) : usize = x
+
+let chacha20_line (a b d: usize) (s: u32) (m: array u32 16sz) : array u32 16sz =
+  let state:array u32 16sz = m in
+  let state:array u32 16sz =
+    state.[ a ] <- Core.Num.wrapping_add_under_impl_8 state.[ a ] state.[ b ]
+  in
+  let state:array u32 16sz = state.[ d ] <- state.[ d ] ^. state.[ a ] in
+  let state:array u32 16sz = state.[ d ] <- Core.Num.rotate_left_under_impl_8 state.[ d ] s in
+  state
+
+let chacha20_quarter_round (a b c d: usize) (state: array u32 16sz) : array u32 16sz =
+  let state:array u32 16sz = chacha20_line a b d 16ul state in
+  let state:array u32 16sz = chacha20_line c d b 12ul state in
+  let state:array u32 16sz = chacha20_line a b d 8ul state in
+  chacha20_line c d b 7ul state
+
+let chacha20_double_round (state: array u32 16sz) : array u32 16sz =
+  let state:array u32 16sz =
+    chacha20_quarter_round (v_BoundedIndex 0sz)
+      (v_BoundedIndex 4sz)
+      (v_BoundedIndex 8sz)
+      (v_BoundedIndex 12sz)
+      state
+  in
+  let state:array u32 16sz =
+    chacha20_quarter_round (v_BoundedIndex 1sz)
+      (v_BoundedIndex 5sz)
+      (v_BoundedIndex 9sz)
+      (v_BoundedIndex 13sz)
+      state
+  in
+  let state:array u32 16sz =
+    chacha20_quarter_round (v_BoundedIndex 2sz)
+      (v_BoundedIndex 6sz)
+      (v_BoundedIndex 10sz)
+      (v_BoundedIndex 14sz)
+      state
+  in
+  let state:array u32 16sz =
+    chacha20_quarter_round (v_BoundedIndex 3sz)
+      (v_BoundedIndex 7sz)
+      (v_BoundedIndex 11sz)
+      (v_BoundedIndex 15sz)
+      state
+  in
+  let state:array u32 16sz =
+    chacha20_quarter_round (v_BoundedIndex 0sz)
+      (v_BoundedIndex 5sz)
+      (v_BoundedIndex 10sz)
+      (v_BoundedIndex 15sz)
+      state
+  in
+  let state:array u32 16sz =
+    chacha20_quarter_round (v_BoundedIndex 1sz)
+      (v_BoundedIndex 6sz)
+      (v_BoundedIndex 11sz)
+      (v_BoundedIndex 12sz)
+      state
+  in
+  let state:array u32 16sz =
+    chacha20_quarter_round (v_BoundedIndex 2sz)
+      (v_BoundedIndex 7sz)
+      (v_BoundedIndex 8sz)
+      (v_BoundedIndex 13sz)
+      state
+  in
+  chacha20_quarter_round (v_BoundedIndex 3sz)
+    (v_BoundedIndex 4sz)
+    (v_BoundedIndex 9sz)
+    (v_BoundedIndex 14sz)
+    state
+
+let chacha20_rounds (state: array u32 16sz) : array u32 16sz =
+  let st:array u32 16sz = state in
+  let st:array u32 16sz =
+    Core.Iter.Traits.Iterator.Iterator.fold (Core.Iter.Traits.Collect.IntoIterator.into_iter ({
+              Core.Ops.Range.Range.f_start = 0sz;
+              Core.Ops.Range.Range.f_end = 10sz
+            }))
+      st
+      (fun st _i -> chacha20_double_round st)
+  in
+  st
+
+let chacha20_core (ctr: u32) (st0: array u32 16sz) : array u32 16sz =
+  let state:array u32 16sz = st0 in
+  let state:array u32 16sz =
+    state.[ 12sz ] <- Core.Num.wrapping_add_under_impl_8 state.[ 12sz ] ctr
+  in
+  let k:array u32 16sz = chacha20_rounds state in
+  Chacha20.Hacspec_helper.add_state state k
+
+let chacha20_init (key: array u8 32sz) (iv: array u8 12sz) (ctr: u32) : array u32 16sz =
+  let (key_u32: array u32 8sz):array u32 8sz =
+    Chacha20.Hacspec_helper.to_le_u32s_8_ (Hax.CoerceUnsize.unsize key)
+  in
+  let (iv_u32: array u32 3sz):array u32 3sz =
+    Chacha20.Hacspec_helper.to_le_u32s_3_ (Hax.CoerceUnsize.unsize iv)
+  in
+  (let l =
+      [
+        1634760805ul; 857760878ul; 2036477234ul; 1797285236ul; key_u32.[ 0sz ]; key_u32.[ 1sz ];
+        key_u32.[ 2sz ]; key_u32.[ 3sz ]; key_u32.[ 4sz ]; key_u32.[ 5sz ]; key_u32.[ 6sz ];
+        key_u32.[ 7sz ]; ctr; iv_u32.[ 0sz ]; iv_u32.[ 1sz ]; iv_u32.[ 2sz ]
+      ]
+    in
+    assert_norm (List.Tot.length l == 16);
+    Hax.Array.array_of_list l)
+
+let chacha20_key_block (state: array u32 16sz) : array u8 64sz =
+  let state:array u32 16sz = chacha20_core 0ul state in
+  Chacha20.Hacspec_helper.u32s_to_le_bytes state
+
+let chacha20_key_block0 (key: array u8 32sz) (iv: array u8 12sz) : array u8 64sz =
+  let state:array u32 16sz = chacha20_init key iv 0ul in
+  chacha20_key_block state
+
+let chacha20_encrypt_block (st0: array u32 16sz) (ctr: u32) (plain: array u8 64sz) : array u8 64sz =
+  let st:array u32 16sz = chacha20_core ctr st0 in
+  let (pl: array u32 16sz):array u32 16sz =
+    Chacha20.Hacspec_helper.to_le_u32s_16_ (Hax.CoerceUnsize.unsize plain)
+  in
+  let encrypted:array u32 16sz = Chacha20.Hacspec_helper.xor_state st pl in
+  Chacha20.Hacspec_helper.u32s_to_le_bytes encrypted
+
+let chacha20_encrypt_last (st0: array u32 16sz) (ctr: u32) (plain: slice u8)
+    : Alloc.Vec.t_Vec u8 Alloc.Alloc.t_Global =
+  let (b: array u8 64sz):array u8 64sz = Hax.Array.repeat 0uy 64sz in
+  let b:array u8 64sz = Chacha20.Hacspec_helper.update_array b plain in
+  let b:array u8 64sz = chacha20_encrypt_block st0 ctr b in
+  Alloc.Slice.to_vec_under_impl b.[ {
+        Core.Ops.Range.RangeTo.f_end = Core.Slice.len_under_impl plain
+      } ]
+
+#push-options "--lax"
+let chacha20_update (st0: array u32 16sz) (m: slice u8) : Alloc.Vec.t_Vec u8 Alloc.Alloc.t_Global =
+  let blocks_out:Alloc.Vec.t_Vec u8 Alloc.Alloc.t_Global = Alloc.Vec.new_under_impl in
+  let num_blocks:usize = Core.Slice.len_under_impl m /. 64sz in
+  let remainder_len:usize = Core.Slice.len_under_impl m %. 64sz in
+  let blocks_out:Alloc.Vec.t_Vec u8 Alloc.Alloc.t_Global =
+    Core.Iter.Traits.Iterator.Iterator.fold (Core.Iter.Traits.Collect.IntoIterator.into_iter ({
+              Core.Ops.Range.Range.f_start = 0sz;
+              Core.Ops.Range.Range.f_end = num_blocks
+            }))
+      blocks_out
+      (fun blocks_out i ->
+          let b:array u8 64sz =
+            chacha20_encrypt_block st0
+              (cast i)
+              (Core.Result.unwrap_under_impl (Core.Convert.TryInto.try_into m.[ {
+                          Core.Ops.Range.Range.f_start = 64sz *. i;
+                          Core.Ops.Range.Range.f_end = 64sz *. i +. 64sz
+                        } ]))
+          in
+          let blocks_out:Alloc.Vec.t_Vec u8 Alloc.Alloc.t_Global =
+            Alloc.Vec.extend_from_slice_under_impl_2 blocks_out (Hax.CoerceUnsize.unsize b)
+          in
+          blocks_out)
+  in
+  let blocks_out:Alloc.Vec.t_Vec u8 Alloc.Alloc.t_Global =
+    if remainder_len <>. 0sz
+    then
+      let b:Alloc.Vec.t_Vec u8 Alloc.Alloc.t_Global =
+        chacha20_encrypt_last st0
+          (cast num_blocks)
+          m.[ { Core.Ops.Range.RangeFrom.f_start = 64sz *. num_blocks } ]
+      in
+      let blocks_out:Alloc.Vec.t_Vec u8 Alloc.Alloc.t_Global =
+        Alloc.Vec.extend_from_slice_under_impl_2 blocks_out (Core.Ops.Deref.Deref.deref b)
+      in
+      blocks_out
+    else blocks_out
+  in
+  blocks_out
+
+let chacha20 (m: slice u8) (key: array u8 32sz) (iv: array u8 12sz) (ctr: u32)
+    : Alloc.Vec.t_Vec u8 Alloc.Alloc.t_Global =
+  let state:array u32 16sz = chacha20_init key iv ctr in
+  chacha20_update state m
